extracted/realistic_diseq_interpreter_wrapped.hs
@@ -1,4 +1,4 @@
-module Obvious_diseq_interpreter where
+module Realistic_diseq_interpreter where
 
 import qualified Prelude as P
 import qualified Data.Maybe
@@ -64,6 +64,16 @@ snd p =
 data List a =
    Nil
  | Cons a (List a)
+
+list_rect :: a2 -> (a1 -> (List a1) -> a2 -> a2) -> (List a1) -> a2
+list_rect f f0 l =
+  case l of {
+   Nil -> f;
+   Cons y l0 -> f0 y l0 (list_rect f f0 l0)}
+
+list_rec :: a2 -> (a1 -> (List a1) -> a2 -> a2) -> (List a1) -> a2
+list_rec =
+  list_rect
 
 app :: (List a1) -> (List a1) -> List a1
 app l m =
@@ -254,7 +264,7 @@ data Stream a =
    Nil0
  | Cons0 a (Stream a)
 
-type Constraint_store = List (Prod Term Term)
+type Constraint_store = List Subst
 
 init_cs :: Constraint_store
 init_cs =
@@ -262,13 +272,57 @@ init_cs =
 
 add_constraint_exists :: Subst -> Constraint_store -> Term -> Term -> SigT
                          (Option Constraint_store) ()
-add_constraint_exists _ cs t1 t2 =
-  ExistT (Some (Cons (Pair t1 t2) cs)) __
+add_constraint_exists s cs t1 t2 =
+  let {mGU_E = mgu_exists (apply_subst s t1) (apply_subst s t2)} in
+  case mGU_E of {
+   ExistT r _ ->
+    case r of {
+     Some s0 ->
+      case s0 of {
+       Nil -> ExistT None __;
+       Cons p s1 -> ExistT (Some (Cons (Cons p s1) cs)) __};
+     None -> ExistT (Some cs) __}}
+
+list_to_term :: (List Term) -> Term
+list_to_term ts =
+  case ts of {
+   Nil -> Cst O;
+   Cons t ts0 -> Con (S O) t (list_to_term ts0)}
+
+upd_constr_exists :: Subst -> Subst -> Subst -> SigT (Option Subst) ()
+upd_constr_exists _ w d =
+  let {
+   mGU_E = mgu_exists
+             (list_to_term
+               (map fst
+                 (map (\p -> Pair (apply_subst d (Var (fst p)))
+                   (apply_subst d (snd p))) w)))
+             (list_to_term
+               (map snd
+                 (map (\p -> Pair (apply_subst d (Var (fst p)))
+                   (apply_subst d (snd p))) w)))}
+  in
+  case mGU_E of {
+   ExistT r _ -> ExistT r __}
 
 upd_cs_exists :: Subst -> Constraint_store -> Subst -> SigT
                  (Option Constraint_store) ()
-upd_cs_exists _ cs _ =
-  ExistT (Some cs) __
+upd_cs_exists s cs d =
+  list_rec (ExistT (Some Nil) __) (\a _ iHcs ->
+    case iHcs of {
+     ExistT rcs' _ ->
+      let {uPD_C_E = upd_constr_exists s a d} in
+      case uPD_C_E of {
+       ExistT rw' _ ->
+        case rcs' of {
+         Some cs' ->
+          case rw' of {
+           Some w' ->
+            case w' of {
+             Nil -> ExistT None __;
+             Cons p w'0 -> ExistT (Some (Cons (Cons p w'0) cs')) __};
+           None -> ExistT (Some cs') __};
+         None -> ExistT None __}}}) cs
 
 data State' =
    Leaf Goal Subst Constraint_store Nat
@@ -608,13 +662,24 @@ streamToList (Cons0 x xs) = x : streamToList xs
 takeValsOnFVs :: P.Int -> Subst -> [Term]
 takeValsOnFVs n s = P.map (\i -> apply_subst s (Var (int_to_nat i))) (P.init [0..n])
 
-interpret :: P.Int -> Goal -> [([Term], List (Term, Term))]
+interpret :: P.Int -> Goal -> [([Term], Constraint_store)]
 interpret n g = let (ExistT t _) = op_sem_exists (State (initial_state g (int_to_nat n)))
-                in P.map (\(Answer s cs _) -> (takeValsOnFVs n s, map (\(Pair t1 t2) -> (apply_subst s t1, apply_subst s t2)) cs))
+                in P.map (\(Answer s cs _) -> (takeValsOnFVs n s, cs))
                          (P.filter answersOnly (streamToList t))
   where
     answersOnly Step = P.False
     answersOnly (Answer _ _ _) = P.True
+
+
+{- newtype ConstraintBinding = ConstraintBinding (Prod Name Term)
+
+instance P.Show ConstraintBinding where
+  show (ConstraintBinding (Pair n v)) = "v" P.++ P.show n P.++ " =/= " P.++ P.show v
+
+show_constraint :: Subst -> P.String
+show_constraint s = P.show P.$ P.map ConstraintBinding P.$ listToPList s -}
+
+
 
 interpretAndPrint :: P.Int -> Goal -> P.IO ()
 interpretAndPrint n g =
@@ -622,14 +687,8 @@ interpretAndPrint n g =
     (\(ans, cs) -> do
       P.putStr (P.show ans)
       P.putStr "\nwith\n"
-      P.mapM_
-        (\(t1, t2) -> do
-          P.putStr (P.show t1)
-          P.putStr " =/= "
-          P.putStr (P.show t2)
-          P.putStr "\n")
-        (listToPList cs)
-      P.putStr "\n")
+      P.mapM_ (\c -> P.putStrLn ("not " P.++ P.show c)) (listToPList cs)
+      P.putStr ";\n\n")
     (interpret n g)
 
 interpretAndPrintFirstK :: P.Int -> P.Int -> Goal -> P.IO ()
@@ -638,13 +697,7 @@ interpretAndPrintFirstK k n g =
     (\(ans, cs) -> do
       P.putStr (P.show ans)
       P.putStr "\nwith\n"
-      P.mapM_
-        (\(t1, t2) -> do
-          P.putStr (P.show t1)
-          P.putStr " =/= "
-          P.putStr (P.show t2)
-          P.putStr "\n")
-        (listToPList cs)
+      P.mapM_ (\c -> P.putStrLn ("not " P.++ P.show c)) (listToPList cs)
       P.putStr ";\n\n")
     (P.take k (interpret n g))
 
