src/ObviousDisequality.v
@@ -14,82 +14,114 @@ Require Import OpSemCompleteness.
 
 Module ObviousConstraintStore <: ConstraintStoreSig.
 
-Definition constraint_store (s : subst) : Set := list (term * term).
+Definition constraint_store : Set := list (term * term).
 
-Definition init_cs : constraint_store empty_subst := [].
 
-Inductive add_constraint_ind_def : forall (s : subst), constraint_store s -> term -> term -> option (constraint_store s) -> Set :=
+Definition in_denotational_sem_cs (s : subst) (cs : constraint_store) (f : repr_fun) :=
+  forall (t1 t2 : term), In (t1, t2) cs -> ~ gt_eq (apply_repr_fun f t1) (apply_repr_fun f t2).
+
+Notation "[| s , cs , f |]" := (in_denotational_sem_cs s cs f) (at level 0).
+
+
+Definition wf_cs (s : subst) (cs : constraint_store) : Prop := True.
+
+
+Definition init_cs : constraint_store := [].
+
+Lemma wf_init_cs : wf_cs empty_subst init_cs.
+Proof. apply I. Qed.
+
+
+Inductive add_constraint_ind_def : subst -> constraint_store -> term -> term -> option constraint_store -> Prop :=
 | acC : forall s cs t1 t2, add_constraint_ind_def s cs t1 t2 (Some ((t1, t2) :: cs)).
 
 Definition add_constraint := add_constraint_ind_def.
 
 Lemma add_constraint_exists :
-  forall (s : subst) (cs : constraint_store s) (t1 t2 : term),
-    {r : option (constraint_store s) & add_constraint s cs t1 t2 r}.
+  forall (s : subst) (cs : constraint_store) (t1 t2 : term),
+    {r : option constraint_store & add_constraint s cs t1 t2 r}.
 Proof. intros. eexists. econstructor. Qed.
 
 Lemma add_constraint_unique :
-  forall (s : subst) (cs : constraint_store s) (t1 t2 : term) (r r' : option (constraint_store s)),
+  forall (s : subst) (cs : constraint_store) (t1 t2 : term) (r r' : option constraint_store),
     add_constraint s cs t1 t2 r -> add_constraint s cs t1 t2 r' -> r = r'.
-Proof. intros. good_inversion H. good_inversion H0. simpl_existT_cs_same. reflexivity. Qed.
+Proof. intros. good_inversion H. good_inversion H0. reflexivity. Qed.
 
-Inductive upd_cs_ind_def : forall (s : subst), constraint_store s -> forall (d : subst), option (constraint_store (compose s d)) -> Set :=
+Lemma add_constraint_wf_preservation :
+  forall (s : subst) (cs : constraint_store) (t1 t2 : term) (cs' : constraint_store),
+    narrowing_subst s ->
+    add_constraint s cs t1 t2 (Some cs') ->
+    wf_cs s cs ->
+    wf_cs s cs'.
+Proof. intros. apply I. Qed.
+
+
+Inductive upd_cs_ind_def : subst -> constraint_store -> subst -> option constraint_store -> Prop :=
 | uC : forall s cs d, upd_cs_ind_def s cs d (Some cs).
 
 Definition upd_cs := upd_cs_ind_def.
 
 Lemma upd_cs_exists :
-  forall (s : subst) (cs : constraint_store s) (d : subst),
-    {r : option (constraint_store (compose s d)) & upd_cs s cs d r}.
+  forall (s : subst) (cs : constraint_store) (d : subst),
+    {r : option constraint_store & upd_cs s cs d r}.
 Proof. intros. eexists. econstructor. Qed.
 
 Lemma upd_cs_unique :
-  forall (s : subst) (cs : constraint_store s) (d : subst) (r r' : option (constraint_store (compose s d))),
+  forall (s : subst) (cs : constraint_store) (d : subst) (r r' : option (constraint_store)),
     upd_cs s cs d r -> upd_cs s cs d r' -> r = r'.
-Proof. intros. good_inversion H. good_inversion H0. simpl_existT_cs_same. reflexivity. Qed.
+Proof. intros. good_inversion H. good_inversion H0. reflexivity. Qed.
 
-Definition in_denotational_sem_cs (s : subst) (cs : constraint_store s) (f : repr_fun) :=
-  forall (t1 t2 : term), In (t1, t2) cs -> ~ gt_eq (apply_repr_fun f t1) (apply_repr_fun f t2).
+Lemma upd_cs_wf_preservation :
+  forall (s : subst) (cs : constraint_store) (d : subst) (cs' : constraint_store),
+    narrowing_subst s ->
+    narrowing_subst d ->
+    extending_subst s d ->
+    upd_cs s cs d (Some cs') ->
+    wf_cs s cs ->
+    wf_cs (compose s d) cs'.
+Proof. intros. apply I. Qed.
 
-Notation "[| s , cs , f |]" := (in_denotational_sem_cs s cs f) (at level 0).
 
 Lemma init_condition : forall f, [| empty_subst , init_cs , f |].
 Proof. unfold in_denotational_sem_cs. contradiction. Qed.
 
 Lemma add_constraint_fail_condition :
-  forall (s : subst) (cs : constraint_store s) (t1 t2 : term),
+  forall (s : subst) (cs : constraint_store) (t1 t2 : term),
+    wf_cs s cs ->
     add_constraint s cs t1 t2 None ->
     forall f, ~ ([| s , cs  , f |] /\ [ s , f ] /\ [| Disunify t1 t2 , f |]).
-Proof. intros. inversion H. Qed.
+Proof. intros. inversion H0. Qed.
 
 Lemma add_constraint_success_condition :
-  forall (s : subst) (cs cs' : constraint_store s) (t1 t2 : term),
+  forall (s : subst) (cs cs' : constraint_store) (t1 t2 : term),
+    wf_cs s cs ->
     add_constraint s cs t1 t2 (Some cs') ->
     forall f, [| s , cs' , f |] /\ [ s , f ] <->
               [| s , cs  , f |] /\ [ s , f ] /\ [| Disunify t1 t2 , f |].
 Proof.
   unfold in_denotational_sem_cs. intros.
-  good_inversion H. simpl_existT_cs_same. good_inversion H4. split.
+  good_inversion H0. split.
   { intros [DSCS DSS]. split; try split; intros; auto.
     { apply DSCS. right. auto. }
     { constructor. apply DSCS. left. auto. }  }
   { intros [DSCS [DSS DSG]]. good_inversion DSG. split; auto. intros.
-    destruct H; auto. good_inversion H; auto. }
+    destruct H0; auto. good_inversion H0; auto. }
 Qed.
 
 Lemma upd_cs_fail_condition :
-  forall (s : subst) (cs : constraint_store s) (d : subst),
+  forall (s : subst) (cs : constraint_store) (d : subst),
+    wf_cs s cs ->
     upd_cs s cs d None -> forall f, ~ ([| s , cs , f |] /\ [ compose s d , f ]).
-Proof. intros. inversion H. Qed.
+Proof. intros. inversion H0. Qed.
 
 Lemma upd_cs_success_condition :
-  forall (s : subst) (cs : constraint_store s) (d : subst) (cs' : constraint_store (compose s d)),
+  forall (s : subst) (cs : constraint_store) (d : subst) (cs' : constraint_store),
+    wf_cs s cs ->
     upd_cs s cs d (Some cs') ->
     forall f, [| compose s d , cs' , f |] /\ [ compose s d , f ] <->
               [| s           , cs  , f |] /\ [ compose s d , f ].
 Proof.
-  unfold in_denotational_sem_cs. intros. good_inversion H. simpl_existT_cs_same.
-  good_inversion H3. reflexivity.
+  unfold in_denotational_sem_cs. intros. good_inversion H0. reflexivity.
 Qed.
 
 End ObviousConstraintStore.
@@ -105,6 +137,6 @@ Import OperationalSemObviousCS.
 
 Extraction Language Haskell.
 
-Extraction "extracted/obvious_diseq_interpreter.hs" op_sem_exists.
+Extraction "extracted/obvious_diseq_interpreter.hs" op_sem_exists initial_state.
 
 
