src/OpSemCompleteness.v
@@ -22,7 +22,7 @@ Lemma search_completeness_generalized
       (g    : goal)
       (CG   : consistent_goal g)
       (s    : subst)
-      (cs   : constraint_store s)
+      (cs   : constraint_store)
       (n    : nat)
       (WF   : well_formed_state' (Leaf g s cs n))
       (t    : trace)
@@ -40,11 +40,11 @@ Proof.
     { good_inversion DSG. }
     { exists f. split.
       { econstructor. eexists. eexists. split; eauto.
-        good_inversion OP. good_inversion EV. simpl_existT_cs_same. constructor. }
+        good_inversion OP. good_inversion EV. constructor. }
       { intros; red; auto. } }
     { exists f. split.
       2: intros; red; auto.
-      good_inversion OP. good_inversion EV; good_inversion DSG; simpl_existT_cs_same.
+      good_inversion OP. good_inversion EV; good_inversion DSG.
       { destruct DSS as [fs COMP_s_fs]. red in UNI.
         rewrite <- (repr_fun_eq_apply _ _ t COMP_s_fs) in UNI.
         rewrite <- (repr_fun_eq_apply _ _ t0 COMP_s_fs) in UNI.
@@ -53,24 +53,24 @@ Proof.
         apply unfier_from_gt_unifier in UNI.
         destruct UNI as [sc [SC_UNIFIES _]]. specialize (mgu_non_unifiable _ _ MGU sc).
         contradiction. }
-      { specialize (upd_cs_fail_condition _ _ _ UPD_CS f).
+      { good_inversion WF. specialize (upd_cs_fail_condition _ _ _ WF_CS UPD_CS f).
         intros C. exfalso. apply C. split; auto.
         apply (denotational_sem_uni _ _ _ _ MGU); auto. }
       { red. exists (compose s d). exists cs'. exists n. split.
         { constructor. }
-        { apply and_comm. specialize (upd_cs_success_condition _ _ _ _ UPD_CS f).
+        { apply and_comm. good_inversion WF. specialize (upd_cs_success_condition _ _ _ _ WF_CS UPD_CS f).
           intro EQUI. apply EQUI. split; auto. apply (denotational_sem_uni _ _ _ _ MGU); auto. } } }
     { exists f. split.
       2: intros; red; auto.
       good_inversion DSG. good_inversion OP.
-      good_inversion EV; simpl_existT_cs_same.
-      { exfalso. eapply add_constraint_fail_condition in ADD_C. eauto. }
+      good_inversion EV.
+      { exfalso. eapply add_constraint_fail_condition in ADD_C. eauto. good_inversion WF. auto. }
       { red. exists s. exists cs'. exists n. split.
         { constructor. }
         { apply and_comm. eapply add_constraint_success_condition in ADD_C.
-          apply ADD_C. auto. } } }
+          apply ADD_C. auto. good_inversion WF. auto. } } }
     { good_inversion OP. inversion EV; subst.
-      apply well_formedness_preservation in EV; auto. good_inversion EV. simpl_existT_cs_same.
+      apply well_formedness_preservation in EV; auto. good_inversion EV.
       good_inversion wfState.
       specialize (op_sem_exists (State (Leaf g1 s cs n))). intro p1. destruct p1 as [t1 OP1].
       specialize (op_sem_exists (State (Leaf g2 s cs n))). intro p2. destruct p2 as [t2 OP2].
@@ -86,19 +86,21 @@ Proof.
         red in HinDA. destruct HinDA as [sr [csr [nr [Hin [DSSr DSCSr]]]]].
         red. exists sr. exists csr. exists nr. split; auto. constructor.
         apply (interleave_in _ _ _ Hinter (Answer sr csr nr)). auto. } }
-    { good_inversion DSG. good_inversion OP. inversion EV; simpl_existT_cs_same; subst.
+    { good_inversion DSG. good_inversion OP. inversion EV; subst.
       specialize (op_sem_exists (State (Leaf g1 s cs n))). intro p1. destruct p1 as [t1 OP1].
       assert (wfst'1 : well_formed_state' (Leaf g1 s cs n)).
-      { constructor; good_inversion WF; simpl_existT_cs_same; auto. }
+      { constructor; good_inversion WF; auto. }
       specialize (IHg1 f s n cs CG_G1 DSG_L DSS DSCS wfst'1 t1 OP1).
       destruct IHg1 as [f' [HinDA ff'_eq]]. red in HinDA.
       destruct HinDA as [s' [cs' [n' [Hinstr' [HDAS' HDACS']]]]].
       specialize (op_sem_exists (State (Leaf g2 s' cs' n'))). intro p2. destruct p2 as [t2 OP2].
       specialize (counter_in_trace _ _ _ _ _ _ _ _ OP1 Hinstr'). intro n_le_n'.
       assert (wfst'2 : well_formed_state' (Leaf g2 s' cs' n')).
-      { good_inversion WF. simpl_existT_cs_same.
+      { good_inversion WF.
         destruct (well_formed_subst_in_trace _ (wfNonEmpty _ wfst'1)  _ OP1 _ _ _ Hinstr').
         specialize (well_formed_ds_in_trace _ (wfNonEmpty _ wfst'1)  _ OP1 _ _ _ Hinstr').
+        specialize (narrowing_subst_in_trace _ (wfNonEmpty _ wfst'1)  _ OP1 _ _ _ Hinstr').
+        specialize (wf_cs_in_trace _ (wfNonEmpty _ wfst'1)  _ OP1 _ _ _ Hinstr').
         intros. constructor; auto. intros.
         apply lt_le_trans with n; auto. }
       assert (Hg2' : in_denotational_sem_lev_goal (S l) g2 f').
@@ -113,7 +115,7 @@ Proof.
       { intros. red. apply eq_trans with (proj1_sig (f' x)).
         { apply ff'_eq. auto. }
         { apply f'f''_eq. omega. } } }
-    { good_inversion DSG. good_inversion OP. inversion EV; simpl_existT_cs_same; subst.
+    { good_inversion DSG. good_inversion OP. inversion EV; subst.
       apply well_formedness_preservation in EV; auto. good_inversion EV.
       rename fn into fa.
       remember (fun x => if name_eq_dec x n
@@ -125,7 +127,7 @@ Proof.
         {  destruct (name_eq_dec n n); try contradiction. reflexivity. }
         { intros. destruct (name_eq_dec x n); try contradiction. auto. } }
       assert (DSSn_AND_DSCSn : [ s , fn ] /\ [| s , cs , fn |]).
-      { good_inversion WF. simpl_existT_cs_same. apply (DS_LT_COUNTER f); auto.
+      { good_inversion WF. apply (DS_LT_COUNTER f); auto.
         intros. destruct (name_eq_dec x n); try omega. reflexivity. }
       destruct DSSn_AND_DSCSn as [DSSn DSCSn].
       specialize (H n fn s (S n) cs (CG_BODY n) Hgn DSSn DSCSn wfState t0 OP0).
@@ -136,7 +138,7 @@ Proof.
         specialize (ff'_eq x H0). red in ff'_eq. red. rewrite <- ff'_eq.
         rewrite Heqfn. destruct (name_eq_dec x n); try omega. reflexivity. } }
     { good_inversion DSG. good_inversion OP. inversion EV; subst.
-      apply well_formedness_preservation in EV; auto. good_inversion EV. simpl_existT_cs_same.
+      apply well_formedness_preservation in EV; auto. good_inversion EV.
       assert (cg_body : consistent_goal (proj1_sig (MiniKanrenSyntax.Prog n) t)).
       { remember (MiniKanrenSyntax.Prog n) as d. destruct d as [rel [Hcl Hco]].
         red in Hco. destruct (Hco t) as [Hcog Hcof]. auto. }
