src/RealisticDisequality.v
@@ -1,0 +1,798 @@
+Require Import List.
+Import ListNotations.
+Require Import Coq.Lists.ListSet.
+Require Import Extraction.
+
+Require Import Unify.
+Require Import MiniKanrenSyntax.
+Require Import Stream.
+Require Import DenotationalSem.
+Require Import OperationalSem.
+Require Import OpSemSoundness.
+Require Import OpSemCompleteness.
+
+
+Module RealisticConstraintStore <: ConstraintStoreSig.
+
+Definition constraint_store : Set := list subst.
+
+
+
+Definition in_denotational_sem_cs (s : subst) (cs : constraint_store) (f : repr_fun) :=
+  forall w, In w cs -> ~ [compose s w, f].
+
+Notation "[| s , cs , f |]" := (in_denotational_sem_cs s cs f) (at level 0).
+
+Lemma ds_cs_append
+      (s : subst)
+      (cs : constraint_store)
+      (w : subst)
+      (f : repr_fun)
+      (DSC : ~ [compose s w, f])
+      (DSCS : [| s , cs , f |]) :
+      [| s , w :: cs , f |].
+Proof.
+  red. intros. destruct H; subst; auto.
+Qed.
+
+Lemma ds_cs_decompose
+      (s : subst)
+      (cs : constraint_store)
+      (w : subst)
+      (f : repr_fun)
+      (DSCS : [| s , w :: cs , f |]) :
+      (~ [compose s w, f]) /\ [| s , cs , f |].
+Proof.
+  red in DSCS. split.
+  { apply DSCS. left. auto. }
+  { red. intros. apply DSCS. right. auto. }
+Qed.
+
+
+
+Definition wf_constraint (s : subst) (w : subst) : Prop := narrowing_subst w /\ extending_subst s w /\ nodup_dom w.
+
+Definition wf_cs (s : subst) (cs : constraint_store) : Prop :=
+  forall w, In w cs -> wf_constraint s w.
+
+Lemma wf_cs_head (s : subst)
+              (w : subst)
+              (cs : constraint_store)
+              (WF : wf_cs s (w :: cs)) :
+              wf_constraint s w.
+Proof. red. intros. apply WF. left. auto. Qed.
+
+Lemma wf_cs_tail (s : subst)
+              (w : subst)
+              (cs : constraint_store)
+              (WF : wf_cs s (w :: cs)) :
+              wf_cs s cs.
+Proof. red. intros. apply WF. right. auto. Qed.
+
+
+
+Definition init_cs : constraint_store := [].
+
+Lemma wf_init_cs : wf_cs empty_subst init_cs.
+Proof. red. intros w C. inversion C. Qed.
+
+
+
+Inductive add_constraint_ind_def : subst -> constraint_store -> term -> term -> option constraint_store -> Prop :=
+| acF : forall s cs t1 t2    (MGU : mgu (apply_subst s t1) (apply_subst s t2) None),
+                             add_constraint_ind_def s cs t1 t2 (Some cs)
+| acE : forall s cs t1 t2    (MGU : mgu (apply_subst s t1) (apply_subst s t2) (Some empty_subst)),
+                             add_constraint_ind_def s cs t1 t2 None
+| acNE : forall s cs t1 t2 w (MGU : mgu (apply_subst s t1) (apply_subst s t2) (Some w))
+                             (W_NEMP : w <> empty_subst),
+                             add_constraint_ind_def s cs t1 t2 (Some (w :: cs)).
+
+Hint Constructors add_constraint_ind_def : core.
+
+Definition add_constraint := add_constraint_ind_def.
+
+Lemma add_constraint_exists :
+  forall (s : subst) (cs : constraint_store) (t1 t2 : term),
+    {r : option constraint_store & add_constraint s cs t1 t2 r}.
+Proof.
+  intros. assert (MGU_E := mgu_exists (apply_subst s t1) (apply_subst s t2)).
+  destruct MGU_E as [r MGU_R]. destruct r.
+  { destruct s0.
+    { exists None. red. auto. }
+    { exists (Some ((p :: s0) :: cs)). red. constructor; auto. intro C; inversion C. } }
+  { exists (Some cs). red. auto. }
+Qed.
+
+Lemma add_constraint_unique :
+  forall (s : subst) (cs : constraint_store) (t1 t2 : term) (r r' : option constraint_store),
+    add_constraint s cs t1 t2 r -> add_constraint s cs t1 t2 r' -> r = r'.
+Proof.
+  intros. good_inversion H; good_inversion H0; auto;
+  assert (eq := mgu_unique _ _ _ _ MGU MGU0); inversion eq; auto.
+  { symmetry in H0. contradiction. }
+  { contradiction. }
+Qed.
+
+Lemma add_constraint_wf_preservation :
+  forall (s : subst) (cs : constraint_store) (t1 t2 : term) (cs' : constraint_store),
+    narrowing_subst s ->
+    add_constraint s cs t1 t2 (Some cs') ->
+    wf_cs s cs ->
+    wf_cs s cs'.
+Proof.
+  intros. good_inversion H0; auto.
+  red in H1. red. intros. destruct H0.
+  { subst. split; try split.
+    { eapply mgu_is_narrowing; eauto. }
+    { eapply mgu_is_extending; eauto. }
+    { eapply mgu_nodup_dom; eauto. } }
+  { apply H1; auto. }
+Qed.
+
+
+Fixpoint list_to_term (ts : list term) : term :=
+  match ts with
+  | [] => Cst 0
+  | t :: ts => Con 1 t (list_to_term ts)
+  end.
+
+Definition mgu_lists (tps : list (term * term)) (r : option subst) : Prop :=
+  mgu (list_to_term (List.map fst tps)) (list_to_term (List.map snd tps)) r.
+
+Definition upd_constr (s : subst) (w : subst) (d : subst) (r : option subst) : Prop :=
+  mgu_lists (List.map (fun p => (apply_subst d (Var (fst p)), apply_subst d (snd p))) w) r.
+
+Lemma upd_constr_exists :
+  forall (s : subst) (w : subst) (d : subst),
+    {r : option subst & upd_constr s w d r}.
+Proof.
+  intros.
+  assert (MGU_E :=
+    mgu_exists
+      (list_to_term (map fst (map (fun p => (apply_subst d (Var (fst p)), apply_subst d (snd p))) w)))
+      (list_to_term (map snd (map (fun p => (apply_subst d (Var (fst p)), apply_subst d (snd p))) w)))).
+  destruct MGU_E as [r MGU_R]. exists r. auto.
+Qed.
+
+Lemma upd_constr_unique :
+  forall (s : subst) (w : subst) (d : subst) (r r' : option subst),
+    upd_constr s w d r -> upd_constr s w d r' -> r = r'.
+Proof.
+  intros.
+  assert (MGU_U :=
+    mgu_unique
+      (list_to_term (map fst (map (fun p => (apply_subst d (Var (fst p)), apply_subst d (snd p))) w)))
+      (list_to_term (map snd (map (fun p => (apply_subst d (Var (fst p)), apply_subst d (snd p))) w)))).
+  apply MGU_U; auto.
+Qed.
+
+Lemma in_dom_monotone
+      (x : name)
+      (s : subst)
+      (y : name)
+      (t : term)
+      (IN_DOM : in_subst_dom s x) :
+      in_subst_dom ((y, t) :: s) x.
+Proof.
+  red. simpl. destruct (PeanoNat.Nat.eq_dec y x).
+  { eexists; eauto. }
+  { auto. }
+Qed.
+
+Lemma in_vran_monotone
+      (x : name)
+      (s : subst)
+      (y : name)
+      (t : term)
+      (NODD : nodup_dom ((y, t) :: s))
+      (IN_VRAN : in_subst_vran s x) :
+      in_subst_vran ((y, t) :: s) x.
+Proof.
+  good_inversion NODD. red. red in IN_VRAN. destruct IN_VRAN as [x' [t' [IMG_x' FV_x_t']]].
+  exists x'. exists t'. simpl. destruct (PeanoNat.Nat.eq_dec y x').
+  { subst. exfalso. apply H1. induction s.
+    { good_inversion IMG_x'. }
+    { destruct a as [x'' t'']. simpl. simpl in IMG_x'.
+      destruct (PeanoNat.Nat.eq_dec x'' x').
+      { left. auto. }
+      { right. apply IHs; auto.
+        { intro IN_x_s. apply H1. simpl. right. auto. }
+        { good_inversion H2. auto. } } } }
+  { split; auto. }
+Qed.
+
+Lemma upd_constr_wf_preservation :
+  forall (s : subst) (w : subst) (d : subst) (w' : subst),
+    narrowing_subst s ->
+    narrowing_subst d ->
+    extending_subst s d ->
+    upd_constr s w d (Some w') ->
+    wf_constraint s w ->
+    wf_constraint (compose s d) w'.
+Proof.
+  intros s w d w' NAR_S NAR_D EXT_SD UPD WF. split; try split.
+  { red in UPD. red in UPD. eapply mgu_is_narrowing; eauto. }
+  { red. red in UPD. red in UPD.
+    remember (list_to_term (map fst (map (fun p => (apply_subst d (Var (fst p)), apply_subst d (snd p))) w))) as lterm1.
+    remember (list_to_term (map snd (map (fun p => (apply_subst d (Var (fst p)), apply_subst d (snd p))) w))) as lterm2.
+    assert (LTERM1_FV : forall x, In x (fv_term lterm1) -> (in_subst_dom w x /\ image d x = None) \/ in_subst_vran d x).
+    { clear WF Heqlterm2 UPD lterm2. revert Heqlterm1. revert lterm1. induction w; intros lterm1 EQ1 x IN_FV.
+      { simpl in EQ1. subst. contradiction. }
+      { simpl in EQ1. rewrite EQ1 in IN_FV. simpl in IN_FV. apply (set_union_elim name_eq_dec) in IN_FV.
+        destruct IN_FV.
+        { destruct a as [y t]. simpl in H. destruct (image d y) eqn:IMG_D.
+          { right. red. eexists; eexists; eauto. }
+          { left. simpl in H. destruct H; try contradiction.
+            subst. split; auto. red. exists t. simpl.
+            destruct (PeanoNat.Nat.eq_dec x x); try contradiction. auto. } }
+        { apply (IHw _ eq_refl) in H. destruct H.
+          { left. destruct H. split; auto. destruct a. eapply in_dom_monotone; eauto. }
+          { right. auto. } } } }
+    assert (LTERM2_FV : forall x, In x (fv_term lterm2) -> (in_subst_vran w x /\ image d x = None) \/ in_subst_vran d x).
+    { destruct WF as [_ [_ NODD_w]]. clear LTERM1_FV Heqlterm1 UPD lterm1. revert Heqlterm2. revert lterm2.
+      induction w; intros lterm2 EQ2 x IN_FV.
+      { simpl in EQ2. subst. contradiction. }
+      { simpl in EQ2. rewrite EQ2 in IN_FV. simpl in IN_FV. apply (set_union_elim name_eq_dec) in IN_FV.
+        destruct IN_FV.
+        { destruct a as [y t]. simpl in H. apply apply_subst_FV_stronger in H.
+          destruct H.
+          { left. destruct H. split; auto.
+            red. exists y. exists t. split; auto.
+            simpl. destruct (PeanoNat.Nat.eq_dec y y); try contradiction. auto. }
+          { right. auto. } }
+        { assert (NODD_w_copy := NODD_w). good_inversion NODD_w. clear H2. rename H3 into NODD_w.
+          apply (IHw NODD_w _ eq_refl) in H. destruct H.
+          { left. destruct H. split; auto. destruct a. eapply in_vran_monotone; eauto. }
+          { right. auto. } } } }
+    assert (LTERMS_DOM_C : forall x, (In x (fv_term lterm1) \/ In x (fv_term lterm2)) ->
+                                     in_subst_dom (compose s d) x -> False).
+    { intros x IN_LTERM12 IN_COMP. apply compose_dom in IN_COMP. red in WF.
+      destruct WF as [NAR_W [EXT_SW _]].
+      red in EXT_SW. destruct EXT_SW as [EXT_SW_DOM EXT_SW_VRAN].
+      red in EXT_SD. destruct EXT_SD as [EXT_SD_DOM EXT_SD_VRAN].
+      red in NAR_W. destruct IN_LTERM12.
+      { apply LTERM1_FV in H. destruct H.
+        { destruct H. destruct IN_COMP.
+          { specialize (EXT_SW_DOM _ H). contradiction. }
+          { red in H1. destruct H1. rewrite H0 in H1. good_inversion H1. } }
+        { destruct IN_COMP.
+          { specialize (EXT_SD_VRAN _ H). contradiction. }
+          { specialize (NAR_D _ H). contradiction. } } }
+      { apply LTERM2_FV in H. destruct H.
+        { destruct H. destruct IN_COMP.
+          { specialize (EXT_SW_VRAN _ H). contradiction. }
+          { red in H1. destruct H1. rewrite H0 in H1. good_inversion H1. } }
+        { destruct IN_COMP.
+          { specialize (EXT_SD_VRAN _ H). contradiction. }
+          { specialize (NAR_D _ H). contradiction. } } } }
+    split.
+    { intros. intro. eapply LTERMS_DOM_C; eauto. eapply mgu_dom;  eauto. }
+    { intros. intro. eapply LTERMS_DOM_C; eauto. eapply mgu_vran; eauto. } }
+  { red in UPD. red in UPD. eapply mgu_nodup_dom; eauto. }
+Qed.
+
+
+
+Inductive upd_cs_ind_def : subst -> constraint_store -> subst -> option constraint_store -> Prop :=
+| uN  : forall s      d,       upd_cs_ind_def s [] d (Some [])
+| uI  : forall s w cs d        (UPD : upd_cs_ind_def s cs d None), 
+                               upd_cs_ind_def s (w :: cs) d None
+| uE  : forall s w cs d        (UPD_C : upd_constr s w d (Some empty_subst)),
+                               upd_cs_ind_def s (w :: cs) d None
+| uF  : forall s w cs d    cs' (UPD_C : upd_constr s w d None)
+                               (UPD : upd_cs_ind_def s cs d (Some cs')),
+                               upd_cs_ind_def s (w :: cs) d (Some cs')
+| uNE : forall s w cs d w' cs' (UPD_C : upd_constr s w d (Some w'))
+                               (W_NEMP : w' <> empty_subst)
+                               (UPD : upd_cs_ind_def s cs d (Some cs')),
+                               upd_cs_ind_def s (w :: cs) d (Some (w' :: cs')).
+
+Hint Constructors upd_cs_ind_def : core.
+
+Definition upd_cs := upd_cs_ind_def.
+
+Lemma upd_cs_exists :
+  forall (s : subst) (cs : constraint_store) (d : subst),
+    {r : option constraint_store & upd_cs s cs d r}.
+Proof.
+  intros. induction cs.
+  { exists (Some []). red. auto. }
+  { destruct IHcs as [rcs' UPD_RCS'].
+    assert (UPD_C_E := upd_constr_exists s a d). destruct UPD_C_E as [rw' UPD_C_RW'].
+    destruct rcs' as [cs' | ].
+    { destruct rw' as [w' | ].
+      { destruct w'.
+        { exists None. red. auto. }
+        { exists (Some ((p :: w') :: cs')). red. apply uNE; auto.
+          intro C. inversion C. } }
+      { exists (Some cs'). red. auto. } }
+    { exists None. red. auto. } }
+Qed.
+
+
+Lemma upd_cs_unique :
+  forall (s : subst) (cs : constraint_store) (d : subst) (r r' : option constraint_store),
+    upd_cs s cs d r -> upd_cs s cs d r' -> r = r'.
+Proof.
+  intros. revert H H0. revert r r'. induction cs; intros r r' UPD_R UPD_R'.
+  { good_inversion UPD_R. good_inversion UPD_R'. auto. }
+  { good_inversion UPD_R; good_inversion UPD_R';
+    try (specialize (IHcs _ _ UPD UPD0); good_inversion IHcs);
+    try (specialize (upd_constr_unique _ _ _ _ _ UPD_C UPD_C0); intro UPD_C_U; good_inversion UPD_C_U);
+    try contradiction; auto. }
+Qed.
+
+Lemma upd_cs_wf_preservation :
+  forall (s : subst) (cs : constraint_store) (d : subst) (cs' : constraint_store),
+    narrowing_subst s ->
+    narrowing_subst d ->
+    extending_subst s d ->
+    upd_cs s cs d (Some cs') ->
+    wf_cs s cs ->
+    wf_cs (compose s d) cs'.
+Proof.
+  intros. revert H2. revert cs'. induction cs; intros; good_inversion H2; auto.
+  { red. intros. good_inversion H2. }
+  { apply IHcs; auto. eapply wf_cs_tail; eauto. }
+  { red. intros. destruct H2.
+    { subst. eapply upd_constr_wf_preservation; eauto. eapply wf_cs_head; eauto. }
+    { eapply IHcs; eauto. eapply wf_cs_tail; eauto. } }
+Qed.
+
+
+
+Lemma init_condition : forall f, [| empty_subst , init_cs , f |].
+Proof. unfold in_denotational_sem_cs. contradiction. Qed.
+
+
+
+Lemma compose_with_empty
+      (s : subst) :
+      compose s empty_subst = s.
+Proof.
+  induction s.
+  { auto. }
+  { unfold compose. destruct a. simpl. rewrite apply_empty.
+    apply f_equal. auto. }
+Qed.
+
+Lemma denotational_sem_uni_fail
+      (s : subst)
+      (t1 t2 : term)
+      (MGU : mgu (apply_subst s t1) (apply_subst s t2) None)
+      (f : repr_fun)
+      (DSS : [ s , f ])
+      (EQ : gt_eq (apply_repr_fun f t1) (apply_repr_fun f t2)) :
+      False.
+Proof.
+  red in DSS. destruct DSS as [f' EQ_f_sf'].
+  assert (gt_eq (apply_repr_fun f' (apply_subst s t1)) (apply_repr_fun f' (apply_subst s t2))).
+  { red. rewrite <- repr_fun_apply_compose. rewrite <- repr_fun_apply_compose.
+    etransitivity.
+    1: etransitivity.
+    2: eapply EQ.
+    2: symmetry.
+    all: eapply repr_fun_eq_apply; eapply EQ_f_sf'. }
+  apply unfier_from_gt_unifier in H. destruct H as [s' [UNI DSS_s']].
+  eapply mgu_non_unifiable; eauto.
+Qed.
+
+(**)
+
+
+Lemma terms_list_apply_subst_proj_swap_1
+      (s : subst)
+      (ts : list (term * term)) :
+      map fst (map (fun p => (apply_subst s (fst p), apply_subst s (snd p))) ts) =
+      map (apply_subst s) (map fst ts).
+Proof. induction ts; auto. simpl. rewrite IHts. auto. Qed.
+
+Lemma terms_list_apply_subst_proj_swap_2
+      (s : subst)
+      (ts : list (term * term)) :
+      map snd (map (fun p => (apply_subst s (fst p), apply_subst s (snd p))) ts) =
+      map (apply_subst s) (map snd ts).
+Proof. induction ts; auto. simpl. rewrite IHts. auto. Qed.
+
+Lemma term_list_apply_subst_swap
+      (s : subst)
+      (ts : list term) :
+      list_to_term (map (apply_subst s) ts) = apply_subst s (list_to_term ts).
+Proof. induction ts; auto. simpl. rewrite IHts. auto. Qed.
+
+Lemma terms_list_repr_fun_unifier_iff
+      (ts : list (term * term))
+      (f : repr_fun) : 
+      gt_eq (apply_repr_fun f (list_to_term (map fst ts))) (apply_repr_fun f (list_to_term (map snd ts))) <->
+      (forall t1 t2, In (t1, t2) ts -> gt_eq (apply_repr_fun f t1) (apply_repr_fun f t2)).
+Proof.
+  induction ts; auto.
+  { split; intros; try contradiction. reflexivity. }
+  { split; intros.
+    { destruct a. destruct H0.
+      { good_inversion H0. simpl in H.
+        destruct (apply_repr_fun f t1). destruct (apply_repr_fun f (list_to_term (map fst ts))).
+        destruct (apply_repr_fun f t2). destruct (apply_repr_fun f (list_to_term (map snd ts))).
+        unfold gt_eq in H. simpl in H. unfold gt_eq. simpl. good_inversion H. auto. }
+      { revert H0. revert t1 t2. rewrite <- IHts. simpl in H.
+        destruct (apply_repr_fun f t). destruct (apply_repr_fun f (list_to_term (map fst ts))).
+        destruct (apply_repr_fun f t0). destruct (apply_repr_fun f (list_to_term (map snd ts))).
+        unfold gt_eq in H. simpl in H. unfold gt_eq. simpl. good_inversion H. auto. } }
+    { destruct a.
+      assert (gt_eq (apply_repr_fun f t) (apply_repr_fun f t0) /\
+              gt_eq (apply_repr_fun f (list_to_term (map fst ts)))
+                    (apply_repr_fun f (list_to_term (map snd ts)))).
+      { rewrite IHts. split.
+        { apply H. left. auto. }
+        { intros. apply H. right. auto. } }
+      destruct H0. simpl.
+      destruct (apply_repr_fun f t). destruct (apply_repr_fun f (list_to_term (map fst ts))).
+      destruct (apply_repr_fun f t0). destruct (apply_repr_fun f (list_to_term (map snd ts))).
+      unfold gt_eq in H0. simpl in H0. unfold gt_eq in H1. simpl in H1. unfold gt_eq. simpl.
+      congruence. } }
+Qed.
+
+Lemma denotational_sem_uni_fail_lists
+      (s : subst)
+      (ts : list (term * term))
+      (MGU : mgu_lists (map (fun p => (apply_subst s (fst p), apply_subst s (snd p))) ts) None)
+      (f : repr_fun)
+      (DSS : [ s , f ])
+      (EQS : forall t1 t2, In (t1, t2) ts -> gt_eq (apply_repr_fun f t1) (apply_repr_fun f t2)) :
+      False.
+Proof.
+  red in MGU.
+  rewrite terms_list_apply_subst_proj_swap_1 in MGU. rewrite terms_list_apply_subst_proj_swap_2 in MGU.
+  do 2 (rewrite term_list_apply_subst_swap in MGU). rewrite <- terms_list_repr_fun_unifier_iff in EQS.
+  eapply denotational_sem_uni_fail; eauto.
+Qed.
+
+Lemma denotational_sem_uni_lists
+      (s d : subst)
+      (ts : list (term * term))
+      (MGU : mgu_lists (map (fun p => (apply_subst s (fst p), apply_subst s (snd p))) ts) (Some d))
+      (f : repr_fun) :
+      [compose s d , f] <-> [s , f] /\
+                            (forall t1 t2, In (t1, t2) ts -> gt_eq (apply_repr_fun f t1) (apply_repr_fun f t2)).
+Proof.
+  red in MGU.
+  rewrite terms_list_apply_subst_proj_swap_1 in MGU. rewrite terms_list_apply_subst_proj_swap_2 in MGU.
+  do 2 (rewrite term_list_apply_subst_swap in MGU). rewrite <- terms_list_repr_fun_unifier_iff.
+  eapply denotational_sem_uni; eauto.
+Qed.
+
+
+Lemma add_constraint_fail_condition :
+  forall (s : subst) (cs : constraint_store) (t1 t2 : term),
+    wf_cs s cs ->
+    add_constraint s cs t1 t2 None ->
+    forall f, ~ ([| s , cs  , f |] /\ [ s , f ] /\ [| Disunify t1 t2 , f |]).
+Proof.
+  intros. good_inversion H0.
+  apply denotational_sem_uni with (f := f) in MGU. rewrite compose_with_empty in MGU.
+  rewrite MGU. intros [_ [[_ UNI] DISUNI]]. good_inversion DISUNI. auto.
+Qed.
+
+Lemma add_constraint_success_condition :
+  forall (s : subst) (cs cs' : constraint_store) (t1 t2 : term),
+    wf_cs s cs ->
+    add_constraint s cs t1 t2 (Some cs') ->
+    forall f, [| s , cs' , f |] /\ [ s , f ] <->
+              [| s , cs  , f |] /\ [ s , f ] /\ [| Disunify t1 t2 , f |].
+Proof.
+  intros. good_inversion H0.
+  { split.
+    { intros [DSCS DSS]. split; try split; auto.
+      constructor. intro EQ. eapply denotational_sem_uni_fail; eauto. }
+    { intros [DSCS [DSS _]]. split; auto. } }
+  { apply denotational_sem_uni with (f := f) in MGU. split.
+    { intros [DSCS DSS]. apply ds_cs_decompose in DSCS.
+      destruct DSCS as [DSC DSCS]. split; try split; auto.
+      constructor. intro EQ. apply DSC. apply MGU. split; auto. }
+    { intros [DSCS [DSS DISEQ]]. split; try split; auto.
+      apply ds_cs_append; auto. rewrite MGU. intros [_ EQ].
+      good_inversion DISEQ. auto. } }
+Qed.
+
+
+Lemma image_var_dom
+      (s : subst)
+      (x : name)
+      (t : term)
+      (NODD : nodup_dom s)
+      (IN : In (x, t) s) :
+      image s x = Some t.
+Proof.
+  red in NODD. induction s; try contradiction.
+  good_inversion NODD. destruct a as [z tz].
+  simpl. destruct (PeanoNat.Nat.eq_dec z x); subst.
+  { destruct IN.
+    { good_inversion H. auto. }
+    { exfalso. apply H1. apply (in_map fst) in H. auto. } }
+  { apply IHs; auto. destruct IN; auto. good_inversion H. contradiction. }
+Qed.
+
+Lemma apply_subst_var_dom
+      (s : subst)
+      (x : name)
+      (t : term)
+      (NODD : nodup_dom s)
+      (IN : In (x, t) s) :
+      apply_subst s (Var x) = t.
+Proof. simpl. rewrite (image_var_dom _ _ _ NODD IN). auto. Qed.
+
+Lemma apply_subst_FV_not_dom
+      (s : subst)
+      (t : term)
+      (FV_ND : forall x : name, In x (fv_term t) -> ~ in_subst_dom s x) :
+      apply_subst s t = t.
+Proof.
+  induction t; auto.
+  { simpl. destruct (image s n) eqn:EQ; auto.
+    exfalso. apply (FV_ND n).
+    { left. auto. }
+    { red. exists t. auto. } }
+  { simpl. rewrite IHt1. 1: rewrite IHt2; auto.
+    { intros. apply FV_ND. simpl. apply (set_union_intro name_eq_dec). right. auto. }
+    { intros. apply FV_ND. simpl. apply (set_union_intro name_eq_dec). left. auto. } }
+Qed.
+
+Lemma ignore_s_for_wf_constraint
+      (s w : subst)
+      (WF : wf_constraint s w)
+      (y : name)
+      (t : term)
+      (IN_w : In (y, t) w) :
+      apply_subst s (Var y) = Var y /\ apply_subst s t = t.
+Proof.
+  red in WF. destruct WF as [_ [EXT NODD]]. destruct EXT as [NDOM_DOM NDOM_VRAN].
+  split.
+  { apply apply_subst_FV_not_dom. intros. destruct H; try contradiction. subst. apply NDOM_DOM.
+    red. exists t. apply image_var_dom; auto. }
+  { apply apply_subst_FV_not_dom. intros. apply NDOM_VRAN.
+    red. exists y. exists t. split; auto. apply image_var_dom; auto. }
+Qed.
+
+Lemma ignore_w_in_ran_for_wf_constraint
+      (s w : subst)
+      (WF : wf_constraint s w)
+      (y : name)
+      (t : term)
+      (IN_w : In (y, t) w) :
+      apply_subst w t = t.
+Proof.
+  red in WF. destruct WF as [NAR [_ NODD]]. red in NAR.
+  apply apply_subst_FV_not_dom. intros. apply NAR.
+  red. exists y. exists t. split; auto.
+  apply image_var_dom; auto.
+Qed.
+
+
+Lemma upd_constr_fail
+      (s w d : subst)
+      (WFC : wf_constraint s w)
+      (UPD_C : upd_constr s w d None)
+      (f : repr_fun)
+      (DSS_sd : [compose s d, f])
+      (DSS_sw : [compose s w, f]) :
+      False.
+Proof.
+  red in UPD_C. remember (map (fun p => (Var (fst p), snd p)) w) as w_v.
+  assert (IN_wv_w : forall t1 t2, In (t1, t2) w_v -> exists y, t1 = Var y /\ In (y, t2) w).
+  { subst. clear WFC DSS_sw UPD_C. induction w; try contradiction.
+    intros. destruct a as [y t]. destruct H.
+    { good_inversion H. exists y. split; auto. left. auto. }
+    { specialize (IHw t1 t2 H). destruct IHw as [y0 [EQ_y0 IN_y0]].
+      exists y0. split; auto. right. auto. } }
+  assert (IGN_s : forall y t, In (y, t) w -> apply_subst s (Var y) = Var y /\ apply_subst s t = t).
+  { intros. eapply ignore_s_for_wf_constraint; eauto. }
+  assert (IGN_w_vran : forall y t, In (y, t) w -> apply_subst w t = t).
+  { intros. eapply ignore_w_in_ran_for_wf_constraint; eauto. }
+  assert (EQ_MAPS : 
+    map (fun p => (apply_subst (compose s d)     (fst p) , apply_subst (compose s d) (snd p))) w_v =
+    map (fun p => (apply_subst            d (Var (fst p)), apply_subst            d  (snd p))) w).
+  { rewrite Heqw_v. clear IGN_w_vran IN_wv_w WFC UPD_C DSS_sw Heqw_v. induction w; auto.
+    destruct a as [y t].
+    Arguments apply_subst : simpl never. simpl.
+    assert (CONJEQ : apply_subst s (Var y) = Var y /\ apply_subst s t = t).
+    { apply IGN_s. left. auto. }
+    destruct CONJEQ as [EQ1 EQ2]. do 2 (rewrite compose_correctness).
+    rewrite EQ1. rewrite EQ2. apply f_equal. apply IHw.
+    intros. apply IGN_s. right. auto. }
+  rewrite <- EQ_MAPS in UPD_C. apply (denotational_sem_uni_fail_lists _ _ UPD_C f); auto.
+  red in DSS_sw. destruct DSS_sw as [f' EQ_swf'_f]. intros t1 t2 IN_wv.
+  etransitivity.
+  1: etransitivity.
+  1: symmetry.
+  1,3: eapply repr_fun_eq_apply; eapply EQ_swf'_f.
+  apply IN_wv_w in IN_wv. destruct IN_wv as [y [EQ_t1 IN_wv]]. subst. 
+  destruct WFC as [_ [_ NODD]]. assert (EQ_n2_t2 := apply_subst_var_dom _ _ _ NODD IN_wv).
+  assert (IN_w := IN_wv). apply IGN_s in IN_wv. destruct IN_wv as [EQ1 EQ2].
+  do 2 (rewrite repr_fun_apply_compose). do 2 (rewrite compose_correctness).
+  rewrite EQ1. rewrite EQ2. simpl. rewrite EQ_n2_t2. apply IGN_w_vran in IN_w.
+  rewrite IN_w. auto.
+Qed.
+
+
+Lemma gt_eq_eq_repr_fun
+      (t1 t2 : term)
+      (f1 f2 : repr_fun)
+      (FEQ : repr_fun_eq f1 f2)
+      (GTEQ : gt_eq (apply_repr_fun f1 t1) (apply_repr_fun f1 t2)) :
+      gt_eq (apply_repr_fun f2 t1) (apply_repr_fun f2 t2).
+Proof.
+  etransitivity.
+  1: etransitivity.
+  2: apply GTEQ.
+  1: symmetry.
+  all: eapply repr_fun_eq_apply; eapply FEQ.
+Qed.
+
+
+Lemma repr_fun_eq_symm
+      (f1 f2 : repr_fun)
+      (EQ : repr_fun_eq f1 f2) :
+      repr_fun_eq f2 f1.
+Proof. red. intros. symmetry. apply EQ. Qed.
+
+Lemma upd_constr_success
+      (s w d w' : subst)
+      (WFC : wf_constraint s w)
+      (UPD_C : upd_constr s w d (Some w'))
+      (f : repr_fun)
+      (DSS_sd : [compose s d, f]) :
+      [compose s w, f] <-> [compose (compose s d) w', f].
+Proof.
+  red in UPD_C. remember (map (fun p => (Var (fst p), snd p)) w) as w_v.
+  assert (IN_w_wv : forall y t, In (y, t) w -> In (Var y, t) w_v).
+  { intros. subst. clear WFC UPD_C. induction w; try contradiction.
+    destruct a as [z tz]. destruct H.
+    { good_inversion H. left. auto. }
+    { apply IHw in H. right. auto. } }
+  assert (IN_wv_w : forall t1 t2, In (t1, t2) w_v -> exists y, t1 = Var y /\ In (y, t2) w).
+  { subst. clear IN_w_wv WFC UPD_C. induction w; try contradiction.
+    intros. destruct a as [y t]. destruct H.
+    { good_inversion H. exists y. split; auto. left. auto. }
+    { specialize (IHw t1 t2 H). destruct IHw as [y0 [EQ_y0 IN_y0]].
+      exists y0. split; auto. right. auto. } }
+  assert (IGN_s : forall y t, In (y, t) w -> apply_subst s (Var y) = Var y /\ apply_subst s t = t).
+  { intros. eapply ignore_s_for_wf_constraint; eauto. }
+  assert (IGN_w_vran : forall y t, In (y, t) w -> apply_subst w t = t).
+  { intros. eapply ignore_w_in_ran_for_wf_constraint; eauto. }
+  assert (EQ_MAPS : 
+    map (fun p => (apply_subst (compose s d)     (fst p) , apply_subst (compose s d) (snd p))) w_v =
+    map (fun p => (apply_subst            d (Var (fst p)), apply_subst            d  (snd p))) w).
+  { rewrite Heqw_v. clear IN_w_wv IGN_w_vran IN_wv_w WFC UPD_C Heqw_v. induction w; auto.
+    destruct a as [y t].
+    Arguments apply_subst : simpl never. simpl.
+    assert (CONJEQ : apply_subst s (Var y) = Var y /\ apply_subst s t = t).
+    { apply IGN_s. left. auto. }
+    destruct CONJEQ as [EQ1 EQ2]. do 2 (rewrite compose_correctness).
+    rewrite EQ1. rewrite EQ2. apply f_equal. apply IHw.
+    intros. apply IGN_s. right. auto. }
+  rewrite <- EQ_MAPS in UPD_C. specialize (denotational_sem_uni_lists _ _ _ UPD_C f). intro EQUI.
+  rewrite EQUI. clear EQ_MAPS EQUI UPD_C.
+  assert (EQUI_ABUND : forall A, [compose s d, f] /\ A <-> A).
+  { intros. split; auto. intros [_ AP]. auto. }
+  rewrite EQUI_ABUND. clear EQUI_ABUND.
+  split.
+  { intros. red in H. destruct H as [f'' EQ_swf''_f].
+    apply IN_wv_w in H0. destruct H0 as [y [EQ_t1 IN_wv]]. subst.
+    apply (gt_eq_eq_repr_fun _ _ _ _ EQ_swf''_f).
+    red. do 2 (rewrite repr_fun_apply_compose). do 2 (rewrite compose_correctness).
+    specialize (IGN_s _ _ IN_wv). destruct IGN_s as [IGN_s_y IGN_s_t2]. specialize (IGN_w_vran _ _ IN_wv).
+    rewrite IGN_s_y. rewrite IGN_s_t2. rewrite IGN_w_vran.
+    destruct WFC as [_ [_ NODD]]. rewrite (apply_subst_var_dom _ _ _ NODD IN_wv). auto. }
+  { intros. red in DSS_sd. destruct DSS_sd as [ff EQ_sdff_f].
+    eapply repr_fun_eq_trans in EQ_sdff_f.
+    2: apply repr_fun_eq_symm; eapply subst_repr_fun_compose_assoc_subst.
+    remember (subst_repr_fun_compose d ff) as f'. clear Heqf'.
+    red. exists f'.
+    eapply repr_fun_eq_trans. 2: eapply EQ_sdff_f.
+    eapply repr_fun_eq_trans. 1: eapply subst_repr_fun_compose_assoc_subst.
+    apply repr_fun_eq_compose. red. intros. unfold subst_repr_fun_compose.
+    assert (CASES := in_dec name_eq_dec x (map fst w)).
+    destruct CASES.
+    { assert (EX_IMG : exists t, In (x, t) w).
+      { clear H IGN_w_vran IGN_s IN_w_wv IN_wv_w Heqw_v WFC. induction w; try contradiction.
+        destruct a as [x0 t]. destruct i.
+        { exists t. left. rewrite <- H. auto. }
+        { apply IHw in H. destruct H as [t1 IN].
+          exists t1. right. auto. } }
+      destruct EX_IMG as [t IN]. assert (IN_w := IN). apply IN_w_wv in IN.
+      apply H in IN. apply repr_fun_eq_symm in EQ_sdff_f.
+      apply (gt_eq_eq_repr_fun _ _ _ _ EQ_sdff_f) in IN.
+      red in IN. do 2 (rewrite repr_fun_apply_compose in IN).
+      destruct WFC as [_ [_ NODD]]. rewrite (apply_subst_var_dom _ _ _ NODD IN_w). symmetry.
+      apply IGN_s in IN_w. destruct IN_w as [EQ1 EQ2].
+      rewrite EQ1 in IN. rewrite EQ2 in IN. auto. }
+    { assert (IGN_w_x : apply_subst w (Var x) = Var x).
+      { clear H IN_w_wv IGN_w_vran IGN_s IN_wv_w Heqw_v WFC. induction w; auto.
+        destruct a as [y t]. unfold apply_subst. simpl.
+        destruct (PeanoNat.Nat.eq_dec y x); subst.
+        { exfalso. apply n. left. auto. }
+        { apply IHw. intro IN. apply n. right. auto. } }
+      rewrite IGN_w_x. reflexivity. } }
+Qed.
+
+
+Lemma upd_cs_fail_condition :
+  forall (s : subst) (cs : constraint_store) (d : subst),
+    wf_cs s cs ->
+    upd_cs s cs d None ->
+    forall f, ~ ([| s , cs , f |] /\ [ compose s d , f ]).
+Proof.
+  intros s cs ds. induction cs.
+  { intros. good_inversion H0. }
+  { intros. good_inversion H0.
+    { intros [DSCS_acs DSS]. eapply IHcs; auto.
+      { apply wf_cs_tail in H. auto. }
+      { split; eauto. apply ds_cs_decompose in DSCS_acs.
+        destruct DSCS_acs as [_ DSCS]. auto. } }
+    { rename H into WF. intros [DSCS_acs DSS].
+      apply wf_cs_head in WF. specialize (upd_constr_success _ _ _ _ WF UPD_C _ DSS).
+      intros EQU. apply ds_cs_decompose in DSCS_acs. destruct DSCS_acs as [NDSS_sa].
+      apply NDSS_sa. apply EQU. rewrite compose_with_empty. auto. } }
+Qed.
+
+Lemma upd_cs_success_condition :
+  forall (s : subst) (cs : constraint_store) (d : subst) (cs' : constraint_store),
+    wf_cs s cs ->
+    upd_cs s cs d (Some cs') ->
+    forall f, [| compose s d , cs' , f |] /\ [ compose s d , f ] <->
+              [| s           , cs  , f |] /\ [ compose s d , f ].
+Proof.
+  intros s cs ds. induction cs.
+  { intros. good_inversion H0. split; intros [A B]; split; auto;
+    unfold in_denotational_sem_cs; contradiction. }
+  { intros. rename H into WF_acs. good_inversion H0.
+    { split; intros [DSCS DSS_sd]; split; auto.
+      { apply ds_cs_append.
+        { apply wf_cs_head in WF_acs. rename a into w.
+          intros DSS_sw. eapply upd_constr_fail; eauto.  }
+        { apply wf_cs_tail in WF_acs.
+          specialize (IHcs _ WF_acs UPD f).
+          assert (CONJ := conj DSCS DSS_sd).
+          apply IHcs in CONJ. destruct CONJ. auto. } }
+      { apply wf_cs_tail in WF_acs.
+        specialize (IHcs _ WF_acs UPD f).
+        apply ds_cs_decompose in DSCS. destruct DSCS as [_ DSCS].
+        assert (CONJ := conj DSCS DSS_sd).
+        apply IHcs in CONJ. destruct CONJ. auto. } }
+    { split; intros [DSCS DSS_sd]; split; auto.
+      { apply ds_cs_append.
+        { apply wf_cs_head in WF_acs. rename WF_acs into WF. rename a into w.
+          intros DSS_sw. specialize (upd_constr_success _ _ _ _ WF UPD_C _ DSS_sd).
+          intros EQU. apply ds_cs_decompose in DSCS. destruct DSCS as [NDSS_sdw' _].
+          apply NDSS_sdw'. apply EQU. auto. }
+        { apply wf_cs_tail in WF_acs.
+          specialize (IHcs _ WF_acs UPD f).
+          apply ds_cs_decompose in DSCS. destruct DSCS as [_ DSCS].
+          assert (CONJ := conj DSCS DSS_sd).
+          apply IHcs in CONJ. destruct CONJ. auto. } }
+      { rename a into w. assert (WF_cs := WF_acs). apply wf_cs_tail in WF_cs.
+        apply wf_cs_head in WF_acs. rename WF_acs into WF.
+        specialize (IHcs _ WF_cs UPD f).
+        apply ds_cs_decompose in DSCS. destruct DSCS as [DSC DSCS].
+        assert (CONJ := conj DSCS DSS_sd).
+        apply IHcs in CONJ. destruct CONJ.
+        apply ds_cs_append; auto. intros DSS_sdw'.
+        specialize (upd_constr_success _ _ _ _ WF UPD_C _ H0). intros EQU.
+        apply DSC. apply EQU. auto. } } }
+Qed.
+
+End RealisticConstraintStore.
+
+
+Module OperationalSemRealisticCS := OperationalSemAbstr RealisticConstraintStore.
+
+Module OperationalSemRealisticCSSoundness := OperationalSemSoundnessAbstr RealisticConstraintStore.
+
+Module OperationalSemRealisticCSCompleteness := OperationalSemCompletenessAbstr RealisticConstraintStore.
+
+Import OperationalSemRealisticCS.
+
+Extraction Language Haskell.
+
+Extraction "extracted/realistic_diseq_interpreter.hs" op_sem_exists initial_state.
+
